

Extensions

$$1 \quad (a+b)^2 = a^2 + 2ab + b^2$$

$$2 \quad (a-b)^2 = a^2 - 2ab + b^2$$

$$3 \quad (a+b)^2 + (a-b)^2 = 2(a^2 + b^2)$$

$$4 \quad (a+b)^2 - (a-b)^2 = 4ab$$

$$5 \quad (a+b)(a-b) = a^2 - b^2$$

$$6 \quad (a+b)^3 = a^3 + b^3 + 3ab(a+b) \\ = a^3 + b^3 + 3a^2b + 3ab^2$$

$$7 \quad (a-b)^3 = a^3 - b^3 - 3ab(a-b) \\ = a^3 - b^3 - 3a^2b + 3ab^2$$

$$8 \quad (a+b+c)^2 = a^2 + b^2 + c^2 + 2ab + 2bc + 2ca \\ = a^2 + b^2 + c^2 + 2(ab+bc+ca)$$

$$9 \quad \left(a + \frac{1}{a}\right)^2 = a^2 + \frac{1}{a^2} + 2$$

$$10 \quad \left(a - \frac{1}{a}\right)^2 = a^2 + \frac{1}{a^2} - 2$$

$$11 \quad \left(a + \frac{1}{a}\right)^2 + \left(a - \frac{1}{a}\right)^2 = 2\left(a^2 + \frac{1}{a^2}\right)$$

$$12 \quad (x+a)(x+b) = x^2 + (a+b)x + ab$$

$$13 \quad (x+a)(x-b) = x^2 + (a-b)x - ab$$

$$14 \quad (a-b)(a-b) = a^2 - (b+b)a + b^2$$

$$15 \quad (a-b)(a-b) = a^2 - (b+b)a + b^2$$

$$17 \quad \frac{a^3+b^3+c^3-3abc}{a^2-b^2-c^2} = (a+b+c)(a^2+b^2+c^2-2ab-2bc-2ca)$$

18

$\hookrightarrow x^2 + 4a$

2
i $\left(\frac{7}{8}x + \frac{4}{5}y\right)^2$

using the identity $(a+b)^2 = a^2 + 2ab + b^2$

$a = \frac{7}{8}x$ and $b = \frac{4}{5}y$

$\therefore \left(\frac{7}{8}x + \frac{4}{5}y\right)^2 = \left(\frac{7}{8}x\right)^2 + 2 \times \frac{7}{8}x \times \frac{4}{5}y + \left(\frac{4}{5}y\right)^2$

$= \frac{49x^2}{64} + \frac{7}{5}xy + \frac{16y^2}{25}$

ii $\left(\frac{2x}{7} - \frac{7y}{4}\right)^2$

using identity $(a-b)^2 = a^2 + b^2 - 2ab$

$\left(\frac{2x}{7} - \frac{7y}{4}\right)^2 = \left(\frac{2x}{7}\right)^2 + \left(\frac{7y}{4}\right)^2 - 2\left(\frac{2x}{7} \times \frac{7y}{4}\right)$

$\therefore \left(\frac{2x}{7} - \frac{7y}{4}\right)^2 = \left(\frac{2}{7}x\right)^2 - 2 \times \frac{2}{7}x \times \frac{7}{4}y + \left(\frac{7}{4}y\right)^2$

$= \frac{4x^2}{49} - xy + \frac{49}{16}y^2$

3 using identity $(a+h)^2 - (a-h)^2$

$$(a+h)^2 - (a-h)^2 = 4ah$$

$$a = \frac{a}{2h} \quad h = \frac{2h}{a}$$

$$\left(\frac{a}{2h} + \frac{2h}{a}\right)^2 - \left(\frac{a}{2h} - \frac{2h}{a}\right)^2$$

$$= 4 \times \frac{a}{2h} \times \frac{2h}{a} = 4$$

$$\left(\frac{a}{2h} + \frac{2h}{a}\right)^2 - \left(\frac{a}{2h} - \frac{2h}{a}\right)^2$$

$$4 - 4 = 0$$

i $(x+y)^2 - (x-y)^2 = 4xy$

$$(x+y)^2 - (x-y)^2 = 4xy$$

$$\left(\frac{7}{2}\right)^2 - (x-y)^2 = 4^2 \times \frac{5}{2}$$

$$\frac{49}{4} - (x-y)^2 = 10$$

$$\frac{49}{4} - \frac{40}{1 \times 4} = (x-y)^2$$

$$\frac{49-40}{4} = (x-y)^2$$

$$11 \quad x^2 - y^2 = (x+y)(x-y)$$

$$= \pm \frac{7}{2} \times \frac{3}{2}$$

$$= \pm \frac{21}{4}$$

$P + 0$

$$(x+y)5 = (x-y)5 + (x+y)5$$

$$(5x+5y)5 = 5x^2$$

$$(5x+5y)5 = 0 + 5x^2$$

$$(5x+5y)5 = 5x^2$$

$$5x+5y = \frac{5x^2}{5}$$

$$5x+5y = x^2$$

500
i

$$\begin{aligned}(a+h)^2 - (a-h)^2 &= 4ah \\(a+h)^2 - (0.9)^2 &= 4 \times 0.36 \\(a+h)^2 - 0.81 &= 1.44 \\(a+h)^2 &= 1.44 + 0.81 \\(a+h)^2 &= 2.25 \\(a+h) &= \pm 1.5\end{aligned}$$

ii

$$\begin{aligned}a^2 - h^2 &= (a+h)(a-h) \\&= \pm 1.5 \times 0.9 \\&= \pm 1.35\end{aligned}$$

6

ix

$$(a+h)^2 + (a-h)^2 = 2(a^2 + h^2)$$

$$6^2 + 4^2 = 2(a^2 + h^2)$$

$$36 + 16 = 2(a^2 + h^2)$$

$$52 = 2(a^2 + h^2)$$

$$\frac{52}{2} = a^2 + h^2$$

$$26 = a^2 + h^2$$

$$ii) (a+h)^2 = a^2 + h^2 + 2ah$$

$$6^2 = 26 + 2ah$$

$$36 - 26 = 2ah$$

$$10 = 2ah$$

$$\frac{10}{2} = ah$$

$$\underline{5 = ah}$$

$$7) \left(a + \frac{1}{a}\right)^2 - \left(a - \frac{1}{a}\right)^2 = 4$$

$$6^2 - \left(a - \frac{1}{a}\right)^2 = 4$$

$$36 - 4 = \left(a - \frac{1}{a}\right)^2$$

$$32 = \left(a - \frac{1}{a}\right)^2$$

$$\sqrt{32} = a - \frac{1}{a}$$

$$\pm \sqrt{16 \times 2} = a - \frac{1}{a}$$

$$\pm 4\sqrt{2} = a - \frac{1}{a}$$

$$ii) (a+h)(a-h) = a^2 - h^2$$

$$\left(a + \frac{1}{a}\right)\left(a - \frac{1}{a}\right) = a^2 - \frac{1}{a^2}$$

$$4x \pm 4\sqrt{2} = a^2 - \frac{1}{a^2}$$

$$\pm 2 \cdot 4\sqrt{2} = a^2 - \frac{1}{a^2}$$

8

$$1) a + \frac{1}{a}$$

$$\left(a + \frac{1}{a}\right)^2 - \left(a - \frac{1}{a}\right)^2 = 4$$

$$\left(a - \frac{1}{a}\right)^2 - 8^2 = 4$$

$$\left(a + \frac{1}{a}\right)^2 = 4 + 64$$

$$\left(a + \frac{1}{a}\right)^2 = 68$$

$$\left(a + \frac{1}{a}\right) = \pm \sqrt{68}$$

$$\left(a + \frac{1}{a}\right) = \pm \sqrt{8}$$

$$\left(a + \frac{1}{a}\right) = \pm \sqrt{4 \times 2}$$

$$\left(a + \frac{1}{a}\right) = \pm 2\sqrt{2}$$

$$\text{ii } \left(a + \frac{1}{a}\right) \left(a - \frac{1}{a}\right) = a^2 - \frac{1}{a^2}$$

$$\pm 2\sqrt{2} \times 8 = a^2 - \frac{1}{a^2}$$

$$\pm 16\sqrt{2} = a^2 - \frac{1}{a^2}$$

$$\text{So } a^2 - \frac{1}{a^2} = \pm 16\sqrt{2}$$

$$4 \left(\frac{a^2}{a} - \frac{1}{a} \right) + \frac{1}{a} = 0$$

$$a - \frac{1}{a} + \frac{1}{a} = 0$$

$$a + \frac{1}{a} = 3$$

$$\text{ii} \left(a + \frac{1}{a}\right)^2 = a^2 + \frac{1}{a^2} + 2$$

$$3^2 = a^2 + \frac{1}{a^2} + 2$$

$$9 - 2 = a^2 + \frac{1}{a^2}$$

$$7 = a^2 + \frac{1}{a^2}$$

$$10 \quad \text{i} \quad \frac{a^2 - 5a - 1}{a} = 0$$

$$\frac{a^2 - 5a - 1}{a} = 0$$

$$a - 5 - \frac{1}{a} = 0$$

$$a - \frac{1}{a} = 5$$

$$\text{iii} \left(a + \frac{1}{a}\right)^3 - \left(a - \frac{1}{a}\right)^3 = 4$$

$$\left(a + \frac{1}{a}\right)^2 - \left(a - \frac{1}{a}\right)^2 = 4$$

$$\left(a + \frac{1}{a}\right)^2 - 5^2 = 4$$

$$\left(a + \frac{1}{a}\right)^2 = 4 + 25$$

$$\left(a + \frac{1}{a}\right)^2 = 4 + 25$$

$$\left(a + \frac{1}{a}\right)^2 = 29$$

$$ii \quad a^2 - \frac{1}{a^2} = (a + \frac{1}{a})(a - \frac{1}{a})$$

$$a^2 - \frac{1}{a^2} = \left(a + \frac{1}{a}\right)\left(a - \frac{1}{a}\right)$$

$$= \pm \sqrt{29 \times 5}$$

$$= \pm 5\sqrt{29}$$

$$ii \quad (3x + 4y) = 16$$

squaring on both sides

$$(3x + 4y)^2 = 16^2$$

$$(3x)^2 + (4y)^2 + 2 \times 3x \times 4y = 256$$

$$9x^2 + 16y^2 + 24xy = 256$$

$$9x^2 + 16y^2 + 24x \times 4 = 256$$

$$9x^2 + 16y^2 = 256 - 96$$

$$9x^2 + 16y^2 = 160$$

12 Let 2 numbers be x and y , $x > y$

$$x - y = 5$$

$$x^2 + y^2 = 73$$

$$\text{to find } x \cdot y$$

$$(x - y)^2 = x^2 + y^2 - 2xy$$

$$5^2 = 73 - 2xy$$

$$25 = 73 - 2xy$$

$$2xy = 73 - 25$$

$$2xy = 48$$

$$xy = \frac{48}{2} = 24$$

Ex 4B

2

2

i $(3a - 2b)^3$

$$(a - b)^3 = a^3 - b^3 - 3ab(a - b)$$

$$a = 3a \quad b = 2b$$

$$\begin{aligned} \therefore (3a - 2b)^3 &= (3a)^3 - (2b)^3 - 3 \times 3a \times 2b(3a - 2b) \\ &= 27a^3 - 8b^3 - 18ab(3a - 2b) \end{aligned}$$

$$= 27a^3 - 8b^3 - 54a^2b + 36ab^2$$

ii $(5a + 3b)^3$

$$(a + b)^3 = a^3 + b^3 + 3ab(a + b)$$

$$a = 5a \quad b = 3b$$

$$(5a + 3b)^3 = (5a)^3 + (3b)^3 + 3 \times 5a \times 3b(5a + 3b)$$

$$a = 5a, h = 3h$$

$$\therefore (5a + 3h)^3 = (5a)^3 + 3 \times 5a \times 3h(5a + 3h) \\ 125a^3 + 27h^3 + 225a^2h + 135ah^2$$

$$\text{iii } \left(2a + \frac{1}{2a}\right)^3$$

$$a = 2a, h = \frac{1}{2a}$$

$$\left(2a + \frac{1}{2a}\right)^3 = (2a)^3 + \left(\frac{1}{2a}\right)^3 + 3 \times 2a \times \frac{1}{2a} \left(2a + \frac{1}{2a}\right)$$

$$8a^3 + \frac{1}{8a^3} + 3 \left(2a + \frac{1}{2a}\right)$$

$$= 8a^3 + \frac{1}{8a^3} + 6a - \frac{3}{2a}$$

$$\text{iv } (a+h)^3 = a^3 + h^3 + 3ah(a+h) \\ (a-h)^3 = a^3 - 3ah(a-h)$$

$$2 \left(a + \frac{1}{a}\right)^3 = a^3 + \frac{1}{a^3} - 3 \times \frac{1}{a} \left(a - \frac{1}{a}\right)$$

$$\left(a - \frac{1}{a}\right)^3 = a^3 - \frac{1}{a^3} - 3 \left(a - \frac{1}{a}\right)$$

$$3 \left(a + \frac{1}{a}\right)^2 = a^2 + \frac{1}{a^2} + 2$$

$$\left(a + \frac{1}{a}\right)^2 = 47 + 2 = 49$$

$$\left(a + \frac{1}{a}\right) = \sqrt{49}$$

$$a + \frac{1}{a} = 7$$

$$\text{ii) } \left(a + \frac{1}{a}\right)^3 = a^3 + \frac{1}{a^3} + 3\left(a + \frac{1}{a}\right)$$

$$7^3 = a^3 + \frac{1}{a^3} + 3 \times 7$$

$$343 - 21 = a^3 + \frac{1}{a^3}$$

$$a^3 + \frac{1}{a^3} = 322$$

4

$$\text{i) } \left(a - \frac{1}{a}\right)^3 = a^3 - \frac{1}{a^3} - 3\left(a - \frac{1}{a}\right)$$

$$\left(a - \frac{1}{a}\right)^2 = 18 - 2 = 16$$

$$\left(a - \frac{1}{a}\right) = \pm 4$$

$$\text{ii) } \left(a - \frac{1}{a}\right)^3 = a^3 - \frac{1}{a^3} - 3\left(a - \frac{1}{a}\right)$$

$$64 = a^3 - \frac{1}{a^3} - 3 \times 4$$

$$64 = a^3 - \frac{1}{a^3} - 12$$

$$64 + 12 = a^3 - \frac{1}{a^3}$$

$$76 = a^3 - \frac{1}{a^3}$$

$$76 = a^3 - \frac{1}{a^3}$$

6 Taking on both sides

$$(a+2h)^3 = 125$$

$$a^3 + (2h)^3 + 3 \times a \times 2h(a+2h) = 125$$

$$a^3 + 8h^3 + 6ah \times 5 = 125$$

$$a^3 + 8h^3 + 30ah = 125$$

7 given $\left(a + \frac{1}{a}\right)^2 = 3$

$$\Rightarrow a + \frac{1}{a} = \pm \sqrt{3}$$

$$\left(a + \frac{1}{a}\right)^3 = a^3 + \frac{1}{a^3} + 3\left(a + \frac{1}{a}\right)$$

$$(\sqrt{3})^3 = a^3 + \frac{1}{a^3} + 3 \times \sqrt{3}$$

$$3\sqrt{3} = a^3 + \frac{1}{a^3}$$

$$\therefore a^3 + \frac{1}{a^3} = 0$$

$$(\sqrt{3})^3 = \sqrt{3} \times \sqrt{3} \times \sqrt{3} = 3\sqrt{3}$$

8 if $a+b+c=0$ then $a^3+b^3+c^3=3abc$
 $a+2b+c=0$ then $a^3+(2b)^3+c^3=3abc$
 $a^3+8b^3+c^3=6abc$

OR
 given, $a+2b+c=0$
 $a+2b=-c$

using on both sides $(a+2b)^3 = (-c)^3$

$$a^3 + (2b)^3 + 3 \times a \times 2b \times (a+2b) = -c^3$$

$$a^3 + 8b^3 + 6ab \times -c = -c^3$$

$$a^3 + 8b^3 + c^3 = 6abc$$

9

i $a^3 - 5^3 - (-4)^3$
 $a^3 + (-5)^3 + (-4)^3$

$$a=9, b=-5, c=-4$$

$$a+b+c=9-5-4=9-9=0$$

if $a+b+c=0$ then $a^3+b^3+c^3=3abc$
 $9^3 + (-5)^3 + (-4)^3 = 3 \times 9 \times -5 \times -4$
 $= 540$

ii $38^3 + (-26)^3 + (-12)^3$
 $a=38, b=-26, c=-12$

$$a+b+c = 38-26-12 = 38-38 = 0$$

$$\therefore 38^3 + (-26)^3 + (-12)^3 = 3 \times 38 \times -26 \times -12$$

$$= 35568$$

12

$$x + \frac{1}{x} = 2$$

$$\left(x + \frac{1}{x}\right)^2 = x^2 + \frac{1}{x^2} + 2$$

$$2^2 - 2 = x^2 + \frac{1}{x^2}$$

$$2^2 - 2 = x^2 + \frac{1}{x^2}$$

$$2 = x^2 + \frac{1}{x^2}$$

$$\left(x + \frac{1}{x}\right)^3 = x^3 + \frac{1}{x^3} + 3\left(x + \frac{1}{x}\right)$$

$$2^3 = x^3 + \frac{1}{x^3} + 3 \times 2$$

$$8 - 6 = x^3 + \frac{1}{x^3}$$

$$\therefore x^3 + \frac{1}{x} = 2$$

$$\left(x + \frac{1}{x}\right)^2 = x^2 + \frac{1}{x} + 2$$

$$\left(x^2 + \frac{1}{x^2}\right)^2 = \left(x^2\right)^2 + \frac{1}{\left(x^2\right)^2} + 2$$

$$2^2 - 2 = x^4 + \frac{1}{x^4}$$

$$\therefore x^4 + \frac{1}{x^4} = 2$$

$$\therefore x^2 + \frac{1}{x^2} = x^3 + \frac{1}{x} + x + \frac{1}{x^4}$$

$$i) (x+y)^2 = x^2 + y^2 + 2xy$$

$$4^2 = x^2 + y^2 + 2 \times 20$$

$$16 - 40 = x^2 + y^2$$

$$\therefore x^2 + y^2 = -24$$

$$ii) (x+y)^3 = x^3 + y^3 + 3xy(x+y)$$

$$9^3 = x^3 + y^3 + 3 \times 20 \times 9$$

$$729 - 540 = x^3 + y^3$$

16 2 kotak pender